\documentclass{article}
\usepackage{anyfontsize}
\usepackage[utf8]{inputenc}
\usepackage[russian]{babel}
\usepackage{amssymb}
\usepackage{mathtools}
\usepackage[left=2cm,right=2cm,
	    top=2cm,bottom=2cm,bindingoffset=0cm]{geometry}
\newcommand\proofend{\begin{flushright}$\blacksquare$\end{flushright}}
\title{Задание 5}
\author{
	Дерюгин Денис, студент 561-й учебной группы
}
\date{\today}


\begin{document}
\maketitle
\large{
	\textbf{Условие:} Доказать, что $\mathcal{F}_N^4(x) = N^2x$.\\
	\\
	\textbf{Доказательство:} \\
	Из формулы обращения: $\sum\limits_{j = 0}^{N - 1} X(j)\omega_N^{jk} = Nx(k)$. \\ \\ \\

	$\mathcal{F}_N^4(x)(j) = \sum\limits_{k = 0}^{N - 1} \mathcal{F}_N^3(x)(k)\omega_N^{-kj} = $ \\ \\
	$ = \sum\limits_{k = 0}^{N - 1} \sum\limits_{l = 0}^{N - 1} \mathcal{F}_N^2(x)(l)\omega_N^{-kl}\omega_N^{-kj} = $ \\ \\
	$ = \sum\limits_{k = 0}^{N - 1} \sum\limits_{l = 0}^{N - 1} \sum\limits_{m = 0}^{N - 1} \mathcal{F}_N(x)(m)\omega_N^{-ml}\omega_N^{-kl}\omega_N^{-kj} = $ \\ \\
	$ = \sum\limits_{k = 0}^{N - 1} \sum\limits_{l = 0}^{N - 1} \sum\limits_{m = 0}^{N - 1} X(m)\omega_N^{-ml}\omega_N^{-kl}\omega_N^{-kj} = $ \\ \\
	$ = \sum\limits_{k = 0}^{N - 1} \sum\limits_{l = 0}^{N - 1} Nx(-l)\omega_N^{-kl}\omega_N^{-kj} = $ \\ \\
	$ = N\sum\limits_{k = 0}^{N - 1} X(-k)\omega_N^{-kj} = $
	$ N^2x(j)$.

	\proofend

}
\end{document}
