\documentclass{article}
\usepackage[utf8]{inputenc}
\usepackage[russian]{babel}
\usepackage{amssymb}
\usepackage{mathtools}
\usepackage[left=1cm,right=1cm,
	    top=1cm,bottom=1cm,bindingoffset=0cm]{geometry}
\newcommand\proofend{\begin{flushright}$\blacksquare$\end{flushright}}
\title{Задание 7}
\author{
	Дерюгин Денис, студент 561-й учебной группы
}
\date{\today}


\begin{document}
\maketitle
\large{
	\textbf{Решение:} \\
	$\dfrac{1}{2} \big [ X(k) + \overline{X}(N - k) \big ] = \dfrac{1}{2} \big [ \sum\limits_{j = 0}^{N - 1} x(j) \omega_N^{-kj} + \overline{\sum\limits_{j = 0}^{N - 1} x(j) \omega_N^{-(N - k)j}}\big ] = $\\
	$= \dfrac{1}{2} \big [ \sum\limits_{j = 0}^{N - 1} x(j) \omega_N^{-kj} + \sum\limits_{j = 0}^{N - 1} \overline{x(j)} \omega_N^{-kj}\big ] = \dfrac{1}{2} \big [ \sum\limits_{j = 0}^{N - 1} (x(j) + \overline{x(j)}) \omega_N^{-kj}\big ] =$\\
	$= \dfrac{1}{2} \big [ \sum\limits_{j = 0}^{N - 1} (a(j) + ib(j) + a(j) - ib(j)) \omega_N^{-kj}\big ] = \sum\limits_{j = 0}^{N - 1} a(j) \omega_N^{-kj} = A(k)$.\\ \\ \\



	$-\dfrac{1}{2} i\big [ X(k) - \overline{X}(N - k) \big ] = -\dfrac{1}{2}i \big [ \sum\limits_{j = 0}^{N - 1} x(j) \omega_N^{-kj} - \overline{\sum\limits_{j = 0}^{N - 1} x(j) \omega_N^{-(N - k)j}}\big ] = $\\
	$= -\dfrac{1}{2} i\big [ \sum\limits_{j = 0}^{N - 1} x(j) \omega_N^{-kj} - \sum\limits_{j = 0}^{N - 1} \overline{x(j)} \omega_N^{-kj}\big ] = -\dfrac{1}{2}i \big [ \sum\limits_{j = 0}^{N - 1} (x(j) - \overline{x(j)}) \omega_N^{-kj}\big ] = $ \\
	$= -\dfrac{1}{2}i \big [ \sum\limits_{j = 0}^{N - 1} (a(j) + ib(j) - a(j) + ib(j)) \omega_N^{-kj}\big ] = -i^2\sum\limits_{j = 0}^{N - 1} b(j) \omega_N^{-kj} = B(k)$.



	\proofend
}
\end{document}
